---
header-includes:
  - \usepackage{listings}
  - \usepackage{qtree}
  - \usepackage{multicol}
---

# CS 321 HW 4

## Robert Detjens

---

## 1. Give context-free grammars that generate the following languages:

\lstset{
  xleftmargin=2em,
  literate={->}{$\rightarrow$}{2}
           {lambda}{$\lambda$}{1}
}

- $L_1 = \{ w \in \{0, 1\}^* | w \text{ contains at least three 1s } \}$

  $G = (\{S, A, B, C\}, \{0, 1\}, S, P)$ where $P =$

  \begin{lstlisting}
  S -> 0S | 1A
  A -> 0A | 1B
  B -> 0B | 1C
  C -> 0C | lambda
  \end{lstlisting}

- $L_2 = \{ w \in \{0, 1\}^* | w = w^R \text{ and } |w| \text{ is even } \}$

  $G = (\{S\}, \{0, 1\}, S, P)$ where $P =$

  \begin{lstlisting}
  S -> 0S0
  S -> 1S1
  S -> lambda
  \end{lstlisting}

- $L_3 = \{ a^i b^j c^k | i, j, k \geq 0, \text{ and } i = j \text{ or } i = k \}$

  $G = (\{S, A, B, C, D\}, \{0, 1\}, S, P)$ where $P =$

  \begin{lstlisting}
  S -> aAc | C
  A -> aAc | B
  B -> bB  | lambda
  C -> aC  | D
  D -> bDc | lambda
  \end{lstlisting}

$\pagebreak$

## 2. Consider the following grammar $G = (\{S, A\}, \{a, b\}, S, P)$ where P is defined below:

\begin{lstlisting}
S -> SS | AAA | lambda
A -> aA | Aa  | b
\end{lstlisting}

### a. Give a left-most derivation for the string abbaba.

\begin{lstlisting}
S -> SS -> AAAS -> aAAAS -> aAaAAS -> abaAAS ababAS -> ababbS -> ababb
\end{lstlisting}

### b. Show that the grammar is ambiguous by exhibiting two distinct derivation trees for some terminal string.

For the string `abaabaaba`, there exist multiple derivation trees:

\begin{multicols}{2}
  \begin{itemize}
    \item \Tree [.S [.A a [.A [.A b ] a ] ] [.A a [.A [.A b ] a ] ] [.A a [.A [.A b ] a ] ] ]
    \item \Tree [.S
                  [.S [.A [.A a [.A [.A b ] a ] ] a ] [.A b ] [.A a [.A a [.A [.A b ] a ] ] ] ]
                  [.S $\lambda$ ]
                ]
  \end{itemize}
\end{multicols}

## 3. Find an s-grammar for $L = \{ a^n b^{n+1} : n \geq 1 \}.$

$G = (\{S, A, B, C\}, \{a, b\}, S, P)$ where $P =$

\begin{lstlisting}
S -> aABC
A -> aAB
A -> lambda
B -> b
C -> b
\end{lstlisting}

$\pagebreak$

## 4. Let $L = \{ a^n b^n : n \geq 0 \}$

### a. Show that $L^2$ is a context-free language.

$L^2 = \{ a^n b^n a^m b^m : n \geq 0, m \geq 0 \}$.

As a context-free language is defines as having a context-free grammar that accepts the language, the grammar $G$ to accept $L^2$ is:

$G = (\{S, A\}, \{a, b\}, S, P)$ where $P =$

\begin{lstlisting}
S -> AA
A -> aAb | lambda
\end{lstlisting}

### b. Show that $L^*$ is a context-free language.

$L^* = \{ (a^n b^n)^m  : n \geq 0, m \geq 0 \}$.

As a context-free language is defines as having a context-free grammar that accepts the language, the grammar $G$ to accept $L^*$ is:

$G = (\{S, A\}, \{a, b\}, S, P)$ where $P =$

\begin{lstlisting}
S -> AS  | lambda
A -> aAb | lambda
\end{lstlisting}

## 5. Prove that context-free languages are closed under star-closure.

Given some context-free language $L$, there exists some context-free grammar $G$ that accepts $L$.

$G$ has some starting variable $S$ by definition of being a grammar.

By replacing the starting variable of $G$ with a new starting variable $T$ with the following production, $G$ will accept 0 or more instances of $L$ -- the definition of a star closure.

\begin{lstlisting}
T -> ST | lambda
\end{lstlisting}
